theories/GraphCore/TensorGraphExpr.v
@@ -23,32 +23,32 @@ Section TensorGraphExpr.
 
 Context {T : Type}.
 
-Let TensorGraph := (TensorHyperGraph T).
+Let TensorGraph := (CospanHyperGraph T).
 
-Implicit Types tg : TensorGraph.
+(* Implicit Types tg : TensorGraph. *)
 
 
 Definition tg_abstracts (tm : Pmap (T * list positive * list positive)) :
   list (Idx * list var * list var) :=
-  (λ k_flu : _*(_*list _*list _), 
-    (k_flu.1, bound <$> k_flu.2.1.2, bound <$> k_flu.2.2)) <$> 
+  (λ k_flu : _*(_*list _*list _),
+    (k_flu.1, bound <$> k_flu.2.1.2, bound <$> k_flu.2.2)) <$>
     (map_to_list tm :> list (positive * (T * list positive * list positive))).
 
-Definition tg_list_to_deltas (is_output : bool) 
+Definition tg_list_to_deltas (is_output : bool)
   (idxs : list positive) : list (var * var) :=
   imap (λ idx input, (free $ bcons is_output (Pos.of_succ_nat idx), bound input))
     idxs.
 
 
-Definition graph_namedtensorlist_semantics (tg : TensorGraph) : namedtensorlist := {|
+Definition graph_namedtensorlist_semantics {n m} (tg : TensorGraph n m) : namedtensorlist := {|
   ntl_sums := elements (vertices tg);
-  ntl_abstracts := tg_abstracts tg.(nodes);
-  ntl_deltas := tg_list_to_deltas false tg.(inputs) 
-    ++ tg_list_to_deltas true tg.(outputs); 
+  ntl_abstracts := tg_abstracts tg.(hedges);
+  ntl_deltas := tg_list_to_deltas false tg.(inputs)
+    ++ tg_list_to_deltas true tg.(outputs);
 |}.
 
 
-(* 
+(*
 Definition graph_tensorlist_semantics (tg : TensorGraph) : tensorlist :=
   mk_tl (const 0%nat <$> internal_edges tg)
     (mk_node (i_internal_edges tg) (i_external_edges tg) <$>
@@ -76,13 +76,13 @@ Definition graph_namedtensorlist_semantics (tg : TensorGraph)
   mk_ntl (zip_with (λ i _, (Pos.of_succ_nat i, O)) int_labs $ internal_edges tg)
     (mk_node (zip int_labs (internal_edges tg))
       (zip ext_labs (external_edges tg)) <$>
-      (map_to_list (nodes tg)).*1).
+      (map_to_list (hedges tg)).*1).
 
 Lemma graph_namedtensorlist_semantics_to_aux tg int_labs ext_labs :
   graph_namedtensorlist_semantics tg int_labs ext_labs =
   graph_namedtensorlist_semantics_aux
     (zip int_labs (internal_edges tg)) (zip ext_labs (external_edges tg))
-    (map_to_list (nodes tg)).*1.
+    (map_to_list (hedges tg)).*1.
 Proof.
   unfold graph_namedtensorlist_semantics, graph_namedtensorlist_semantics_aux.
   rewrite fmap_zip_with.
@@ -93,15 +93,15 @@ Qed.
 Definition graph_tabst (tg : TensorGraph) : Pmap (nat * nat) :=
   kmap Pos.of_succ_nat $
   map_imap (λ (k : nat) (_ : T), Some (length (filter (is_node_input k) (edges tg)),
-    length (filter (is_node_output k) (edges tg)))) (nodes tg).
+    length (filter (is_node_output k) (edges tg)))) (hedges tg).
 
 
 Lemma fold_internal_edges tg :
-  filter (is_internal (nodes tg)) (edges tg) = internal_edges tg.
+  filter (is_internal (hedges tg)) (edges tg) = internal_edges tg.
 Proof. reflexivity. Qed.
 
 Lemma fold_external_edges tg :
-  filter (not_internal (nodes tg)) (edges tg) = external_edges tg.
+  filter (not_internal (hedges tg)) (edges tg) = external_edges tg.
 Proof. reflexivity. Qed.
 
 Lemma fold_num_internals tg :
@@ -201,46 +201,114 @@ Lemma uncurry_alt {A B C} (f : A -> B -> C) p :
   uncurry f p = f p.1 p.2.
 Proof.
   now destruct p.
-Qed.
+Qed.*)
 
-Lemma graph_namedtensorlist_semantics_WF tg int_lab ext_lab :
-  NoDup int_lab -> length int_lab = num_internals tg ->
-  WF_ntl (graph_namedtensorlist_semantics tg int_lab ext_lab).
+Lemma list_omap_fmap {A B C} (f : A -> B) (g : B -> option C) (l : list A) :
+  omap g (f <$> l) = omap (g ∘ f) l.
 Proof.
-  intros Hdupi Hleni.
-  split.
-  - cbn.
-    rewrite zip_with_zip.
-    erewrite (list_fmap_ext (uncurry _ )) by now intros; rewrite uncurry_alt.
-    rewrite <- list_fmap_compose.
-    unfold compose; cbn.
-    setoid_rewrite (list_fmap_compose fst Pos.of_succ_nat).
-    rewrite fst_zip by now apply eq_reflexivity.
-    apply NoDup_fmap_2; [apply _|done].
-  - intros r.
-    rewrite elem_of_abstracts_rel_vars, elem_of_list_to_set.
-    cbn -[internal_edges external_edges].
-    intros (f & low & up & (k & [= -> -> ->] & Hk)%elem_of_list_fmap & Hi).
-    apply (elem_of_list_to_set (C:=gset nat)) in Hk.
-    rewrite <- dom_alt in Hk.
-    apply (list_subseteq_app (input_edges_subseteq_labels _ _ _)
-      (output_edges_subseteq_labels _ _ _)) in Hi.
-    rewrite Permutation_swap_app_app, elem_of_app in Hi.
-    destruct Hi as [Hi|HF]. 2:{
-      rewrite !Combinators.compose_assoc in HF.
-      rewrite 2 (list_fmap_compose _ loc), <- fmap_app in HF.
-      apply elem_of_list_fmap in HF as (? & [=] & _).
-    }
-    revert Hi.
-    rewrite elem_of_app, (or_idemp _).
-    rewrite Combinators.compose_assoc, list_fmap_compose.
-    rewrite elem_of_list_fmap_inj by apply _.
-    unfold i_internal_edges, enumerate.
-    rewrite 2 fmap_zip_with.
-    easy.
+  induction l; [done|cbn]; case_match; f_equal; easy.
 Qed.
 
-Lemma relabel_rels_node_input_edges lint k fint :
+Lemma abstracts_bound_vars_graph {n m} (tg : TensorGraph n m) :
+  abstracts_bound_vars (graph_namedtensorlist_semantics tg).(ntl_abstracts) =
+  list_to_set ('(_, low, up) ← (map_to_list tg.(hedges)).*2; low ++ up).
+Proof.
+  cbn.
+  f_equiv.
+  unfold tg_abstracts.
+  rewrite 2 list_fmap_bind.
+  apply list_bind_ext; [|done].
+  intros [k [[idx low] up]].
+  cbn.
+  rewrite <- fmap_app, list_omap_fmap.
+  unfold compose; cbn.
+  rewrite <- list_fmap_alt.
+  apply list_fmap_id.
+Qed.
+
+
+Lemma deltas_bound_vars_graph {n m} (tg : TensorGraph n m) :
+  deltas_bound_vars (graph_namedtensorlist_semantics tg).(ntl_deltas) =
+  list_to_set ((vec_to_list tg.(inputs)) ++ (vec_to_list tg.(outputs))).
+Proof.
+  cbn.
+  rewrite bind_app.
+  unfold tg_list_to_deltas.
+  rewrite 2 imap_to_zip_with_seq.
+  rewrite <- (fmap_zip_with pair
+    (prod_map (free ∘ bcons false ∘ Pos.of_succ_nat) bound)),
+    <- (fmap_zip_with pair
+    (prod_map (free ∘ bcons true ∘ Pos.of_succ_nat) bound)).
+  rewrite 2 list_fmap_bind.
+  unfold compose, prod_map; cbn.
+  now rewrite <- 2 list_fmap_to_bind, 2 snd_zip by now rewrite length_seq.
+Qed.
+
+Lemma abstracts_free_vars_graph {n m} (tg : TensorGraph n m) :
+  abstracts_free_vars (graph_namedtensorlist_semantics tg).(ntl_abstracts) =
+  ∅.
+Proof.
+  cbn.
+  unfold tg_abstracts.
+  rewrite list_fmap_bind.
+  erewrite (list_bind_ext _ (λ _, nil)); [..|reflexivity]. 2:{
+    intros [k [[f low] up]].
+    cbn.
+    rewrite <- fmap_app, list_omap_fmap.
+    unfold compose; cbn.
+    apply elem_of_nil_inv.
+    now intros ? (?&?&?)%elem_of_list_omap.
+  }
+  now rewrite list_bind_nil_r.
+Qed.
+
+Lemma deltas_free_vars_graph {n m} (tg : TensorGraph n m) :
+  deltas_free_vars (graph_namedtensorlist_semantics tg).(ntl_deltas) =
+  list_to_set ((bcons false <$> pseq 1 (N.of_nat n)) ++
+    (bcons true <$> pseq 1 (N.of_nat m))).
+Proof.
+  cbn.
+  rewrite bind_app.
+  unfold tg_list_to_deltas.
+  rewrite 2 imap_to_zip_with_seq.
+  rewrite <- (fmap_zip_with pair
+    (prod_map (free ∘ bcons false ∘ Pos.of_succ_nat) bound)),
+    <- (fmap_zip_with pair
+    (prod_map (free ∘ bcons true ∘ Pos.of_succ_nat) bound)).
+  rewrite 2 list_fmap_bind.
+  unfold compose, prod_map; cbn -[bcons].
+  rewrite <- (list_fmap_to_bind (bcons false ∘ Pos.of_succ_nat ∘ @fst _ Idx)).
+  rewrite <- (list_fmap_to_bind (bcons true ∘ Pos.of_succ_nat ∘ @fst _ Idx)).
+  rewrite 2 (list_fmap_compose fst), 2 fst_zip by now rewrite length_seq.
+  rewrite 2 list_fmap_compose, 2 pseq_to_seq_inv.
+  rewrite 2 length_vec_to_list.
+  reflexivity.
+Qed.
+
+
+Lemma graph_namedtensorlist_semantics_WF {n m} (tg : TensorGraph n m) :
+  WF_ntl (graph_namedtensorlist_semantics tg).
+Proof.
+  split; [|split].
+  - cbn.
+    apply NoDup_elements.
+  - rewrite abstracts_bound_vars_graph.
+    cbn.
+    unfold vertices.
+    rewrite list_to_set_elements.
+    rewrite list_fmap_bind.
+    etransitivity; [|apply union_subseteq_l].
+    apply list_to_set_subseteq.
+    apply eq_reflexivity, list_bind_ext; [|done].
+    now intros [? [[]]].
+  - rewrite deltas_bound_vars_graph.
+    cbn.
+    unfold vertices.
+    rewrite list_to_set_elements.
+    apply union_subseteq_r.
+Qed.
+
+Lemma relabel_bounds_node_input_edges lint k fint :
   prod_map fint id <$>
     (node_input_edges k lint) =
   node_input_edges k (prod_map fint id <$> lint).
@@ -250,7 +318,7 @@ Proof.
   reflexivity.
 Qed.
 
-Lemma relabel_rels_node_output_edges lext k fint :
+Lemma relabel_bounds_node_output_edges lext k fint :
   prod_map fint id <$>
     (node_output_edges k lext) =
   node_output_edges k (prod_map fint id <$> lext).
@@ -259,320 +327,192 @@ Proof.
   rewrite list_filter_fmap.
   reflexivity.
 Qed.
-
-Lemma relabel_rels_input_edges lint lext k fint :
-  relabel_rels (Pos.of_succ_nat ∘ fint ∘ pos_to_nat_pred) <$>
+(*
+Lemma relabel_bounds_input_edges lint lext k fint :
+  relabel_bounds (Pos.of_succ_nat ∘ fint ∘ pos_to_nat_pred) <$>
     (input_edges lint lext k) =
   input_edges (prod_map fint id <$> lint) lext k.
 Proof.
   unfold input_edges.
-  rewrite <- relabel_rels_node_input_edges.
+  rewrite <- relabel_bounds_node_input_edges.
   rewrite <- list_fmap_compose, fmap_app, <- !list_fmap_compose.
   f_equal.
   now apply list_fmap_ext; intros _ ? _; cbn; rewrite pos_to_nat_pred_of_nat.
 Qed.
 
-Lemma relabel_rels_output_edges lint lext k fint :
-  relabel_rels (Pos.of_succ_nat ∘ fint ∘ pos_to_nat_pred) <$>
+Lemma relabel_bounds_output_edges lint lext k fint :
+  relabel_bounds (Pos.of_succ_nat ∘ fint ∘ pos_to_nat_pred) <$>
     (output_edges lint lext k) =
   output_edges (prod_map fint id <$> lint) lext k.
 Proof.
   unfold output_edges.
-  rewrite <- relabel_rels_node_output_edges.
+  rewrite <- relabel_bounds_node_output_edges.
   rewrite <- list_fmap_compose, fmap_app, <- !list_fmap_compose.
   f_equal.
   now apply list_fmap_ext; intros _ ? _; cbn; rewrite pos_to_nat_pred_of_nat.
-Qed.
+Qed. *)
 
-
-Lemma relabel_rels_mk_node lint lext k fint :
-  relabel_abs (relabel_rels (Pos.of_succ_nat ∘ fint ∘ pos_to_nat_pred))
+(*
+Lemma relabel_bounds_mk_node lint lext k fint :
+  relabel_abs (relabel_bounds (Pos.of_succ_nat ∘ fint ∘ pos_to_nat_pred))
     (mk_node lint lext k) =
   mk_node (prod_map fint id <$> lint) lext k.
 Proof.
   unfold mk_node; cbn.
-  now rewrite relabel_rels_input_edges, relabel_rels_output_edges.
-Qed.
+  now rewrite relabel_bounds_input_edges, relabel_bounds_output_edges.
+Qed. *)
 
 
-Lemma relabel_rels_input_edges' lint lext k fr :
-  relabel_rels fr <$>
+(* Lemma relabel_bounds_input_edges' lint lext k fr :
+  relabel_bounds fr <$>
     (input_edges lint lext k) =
   input_edges (prod_map (pos_to_nat_pred ∘ fr ∘ Pos.of_succ_nat) id <$> lint) lext k.
 Proof.
-  rewrite <- relabel_rels_input_edges.
-  apply list_fmap_ext; intros _ ? _; apply relabel_rels_ext; intros ?;
+  rewrite <- relabel_bounds_input_edges.
+  apply list_fmap_ext; intros _ ? _; apply relabel_bounds_ext; intros ?;
   unfold compose; cbn; now rewrite !pos_to_nat_pred_to_pos.
 Qed.
 
-Lemma relabel_rels_output_edges' lint lext k fr :
-  relabel_rels fr <$>
+Lemma relabel_bounds_output_edges' lint lext k fr :
+  relabel_bounds fr <$>
     (output_edges lint lext k) =
   output_edges (prod_map (pos_to_nat_pred ∘ fr ∘ Pos.of_succ_nat) id <$> lint) lext k.
 Proof.
-  rewrite <- relabel_rels_output_edges.
-  apply list_fmap_ext; intros _ ? _; apply relabel_rels_ext; intros ?;
+  rewrite <- relabel_bounds_output_edges.
+  apply list_fmap_ext; intros _ ? _; apply relabel_bounds_ext; intros ?;
   unfold compose; cbn; now rewrite !pos_to_nat_pred_to_pos.
 Qed.
 
-Lemma relabel_rels_mk_node' lint lext k fr :
-  relabel_abs (relabel_rels fr)
+Lemma relabel_bounds_mk_node' lint lext k fr :
+  relabel_abs (relabel_bounds fr)
     (mk_node lint lext k) =
   mk_node (prod_map (pos_to_nat_pred ∘ fr ∘ Pos.of_succ_nat) id <$> lint) lext k.
 Proof.
   unfold mk_node; cbn.
-  now rewrite relabel_rels_input_edges', relabel_rels_output_edges'.
+  now rewrite relabel_bounds_input_edges', relabel_bounds_output_edges'.
+Qed. *)
+
+
+Lemma fmap_elements `{FinSet A SA, FinSet B SB} (f : A -> B) `{!Inj eq eq f} (X : SA) :
+  f <$> elements X ≡ₚ
+  elements (set_map f X :> SB).
+Proof.
+  apply NoDup_Permutation;
+  [apply (NoDup_fmap_2 _ _), NoDup_elements|apply NoDup_elements|].
+  set_solver.
 Qed.
 
 
 
-Lemma graph_namedtensorlist_semantics_reindex_int
-  (fint : nat -> nat) `{Hfint : !Inj eq eq fint} tg int_lab ext_lab :
-  graph_namedtensorlist_semantics tg (fint <$> int_lab) ext_lab =ntl=
-  graph_namedtensorlist_semantics tg int_lab ext_lab.
+Lemma graph_namedtensorlist_semantics_relabel_graph
+  (f : Idx -> Idx) `{Hfint : !Inj eq eq f} {n m} (tg : TensorGraph n m) :
+  graph_namedtensorlist_semantics (relabel_graph f tg) =ntl=
+  graph_namedtensorlist_semantics tg.
 Proof.
-  (* intros Hdupi Hleni. *)
   symmetry.
-  hnf.
-  exists (Pos.of_succ_nat ∘ fint ∘ pos_to_nat_pred).
-  split; [intros ????; apply (inj _)|].
-  split.
-  - cbn -[internal_edges].
-    rewrite fmap_zip_with, zip_with_fmap_l.
+  exists f.
+  split; [intros ? ? ? ?; apply Hfint|].
+  split; [|split].
+  - cbn.
+    rewrite vertices_relabel_graph.
+    now rewrite <- (fmap_elements _).
+  - cbn.
+    unfold tg_abstracts.
+    rewrite map_to_list_fmap, <- 2 list_fmap_compose.
+    apply eq_reflexivity, list_fmap_ext; intros _ [k [[idx low] up]] _.
     cbn.
-    apply eq_reflexivity, zip_with_ext; now intros;
-    rewrite ?pos_to_nat_pred_of_nat.
-  - cbn -[internal_edges external_edges].
-    apply eq_reflexivity.
-    rewrite <- list_fmap_compose.
-    apply list_fmap_ext; intros _ k _.
-    unfold compose at 1.
-    rewrite relabel_rels_mk_node.
-    now rewrite fmap_zip_with, zip_with_fmap_l.
+    rewrite <- 4 list_fmap_compose.
+    reflexivity.
+  - cbn.
+    unfold tg_list_to_deltas.
+    rewrite fmap_app, 2 fmap_imap.
+    rewrite 2 vec_to_list_map, 2 imap_fmap.
+    reflexivity.
 Qed.
 
-Arguments internal_edges !_ /.
-Arguments external_edges !_ /.
 
-Lemma internal_external_decomp tg :
-  edges tg ≡ₚ internal_edges tg ++ external_edges tg.
+Lemma graph_namedtensorlist_semantics_reindex_graph
+  (f : Idx -> Idx) `{Hfint : !Inj eq eq f} {n m} (tg : TensorGraph n m) :
+  graph_namedtensorlist_semantics (reindex_graph f tg) =ntl=
+  ntl_relabel_absidx f (graph_namedtensorlist_semantics tg).
 Proof.
-  unfold internal_edges, external_edges.
-  symmetry.
-  apply filter_with_neg_Permutation.
+  unfold graph_namedtensorlist_semantics, ntl_relabel_absidx; cbn.
+  rewrite (vertices_reindex_graph _).
+  apply ntl_aeq_of_perm; [done| |done].
+  cbn.
+  unfold tg_abstracts.
+  unfold kmap.
+  rewrite map_to_list_to_map by now
+    rewrite fsts_prod_map, (NoDup_fmap _); apply NoDup_fst_map_to_list.
+  rewrite <- 2 list_fmap_compose.
+  reflexivity.
 Qed.
 
-Lemma mk_node_abst_WT'_aux tg int_lab ext_lab k :
-  (num_internals tg <= length int_lab)%nat ->
-  (num_externals tg <= length ext_lab)%nat ->
-  k ∈ dom (nodes tg) ->
-  abst_WT' (graph_tabst tg)
-    (mk_node (zip int_lab (internal_edges tg)) (zip ext_lab (external_edges tg))
-      k).
+Lemma abstracts_bound_vars_ntl_relabel_absidx f ntl :
+  abstracts_bound_vars (ntl_relabel_absidx f ntl).(ntl_abstracts) =
+  abstracts_bound_vars ntl.(ntl_abstracts).
 Proof.
-  intros Hilab Helab Hk.
-  unfold abst_WT';
+  apply set_eq.
+  intros r.
+  rewrite 2 elem_of_abstracts_bound_vars.
   cbn.
-  unfold graph_tabst.
-  rewrite lookup_kmap by apply _.
-  rewrite map_lookup_imap.
-  apply elem_of_dom in Hk as [t Ht].
-  rewrite Ht.
+  setoid_rewrite elem_of_list_fmap.
+  setoid_rewrite exists_pair.
+  setoid_rewrite exists_pair.
   cbn.
-  f_equal.
-  rewrite internal_external_decomp, 2 filter_app.
-  unfold input_edges, output_edges.
-  rewrite !length_app, ! length_fmap.
-  rewrite <- ! length_app.
-  unfold node_input_edges, node_output_edges.
-  rewrite <- 4 filter_app.
-  f_equal; symmetry;
-  rewrite <- (length_fmap snd), <- list_filter_fmap, fmap_app, 2 snd_zip by easy;
+  setoid_rewrite pair_eq.
+  setoid_rewrite pair_eq.
+  naive_solver.
+Qed.
+
+Lemma deltas_bound_vars_ntl_relabel_absidx f ntl :
+  deltas_bound_vars (ntl_relabel_absidx f ntl).(ntl_deltas) =
+  deltas_bound_vars ntl.(ntl_deltas).
+Proof.
   reflexivity.
 Qed.
 
 
-Lemma mk_node_abst_WT'_imap_pair tg k :
-  k ∈ dom (nodes tg) ->
-  abst_WT' (graph_tabst tg)
-    (mk_node (imap pair (internal_edges tg)) 
-      (imap pair (external_edges tg))
-      k).
+
+Lemma ntl_relabel_absidx_aeq f `{Hf : !Inj eq eq f} ntl ntl' :
+  ntl =ntl= ntl' ->
+  ntl_relabel_absidx f ntl =ntl=
+  ntl_relabel_absidx f ntl'.
 Proof.
-  intros Hk.
-  rewrite 2 imap_to_zip_with_seq.
-  apply mk_node_abst_WT'_aux; now try rewrite length_seq.
-Qed.
-
-Import SetoidList SetoidPermutation list.
-
-
-Lemma input_edges_perm_eq lint lint' lext lext' k :
-  lint ≡ₚ lint' -> lext ≡ₚ lext' ->
-  input_edges lint lext k ≡ₚ input_edges lint' lext' k.
-Proof.
-  intros Hlint Hlext.
-  unfold input_edges.
-  do 2 f_equiv;
-  unfold node_input_edges;
-  now f_equiv.
-Qed.
-
-Lemma output_edges_perm_eq lint lint' lext lext' k :
-  lint ≡ₚ lint' -> lext ≡ₚ lext' ->
-  output_edges lint lext k ≡ₚ output_edges lint' lext' k.
-Proof.
-  intros Hlint Hlext.
-  unfold output_edges.
-  do 2 f_equiv;
-  unfold node_output_edges;
-  now f_equiv.
-Qed.
-
-Lemma mk_node_perm_eq lint lint' lext lext' k :
-  lint ≡ₚ lint' -> lext ≡ₚ lext' ->
-  mk_node lint lext k ≡abs≡ₚ mk_node lint' lext' k.
-Proof.
-  intros Hlint Hext.
-  unfold mk_node; cbn.
-  split_and!; cbn;
-  [done|now apply input_edges_perm_eq|now apply output_edges_perm_eq].
-Qed.
-
-(* FIXME: Move *)
-Lemma zip_Permutation_l_exists_r {A B} (l l' : list A) (k : list B) :
-  l ≡ₚ l' ->
-  length l = length k ->
-  exists k', k ≡ₚ k' /\
-  zip l k ≡ₚ zip l' k'.
-Proof.
-  intros Hl.
-  revert k;
-  induction Hl; intros k.
-  - destruct k; [|done].
-    now exists [].
-  - destruct k as [|y k]; [done|].
-    intros [= (k' & Hk & Hzip)%IHHl].
-    exists (y :: k').
-    split; now cbn; f_equiv.
-  - destruct k as [|y' [|x' k]]; [done..|].
-    intros _.
-    exists (x' :: y' :: k).
-    split; cbn; solve_Permutation.
-  - intros Hlen.
-    apply IHHl1 in Hlen as Hk'.
-    destruct Hk' as (k' & Hkk' & Hzip).
-    pose proof Hlen as Hlen'.
-    rewrite Hl1, Hkk' in Hlen'.
-    apply IHHl2 in Hlen' as (k'' & Hk'k'' & Hzip').
-    exists k''.
-    split; solve [eauto using Permutation_trans].
-Qed.
-Lemma zip_Permutation_r_exists_l {A B} (l : list A) (k k' : list B) :
-  k ≡ₚ k' ->
-  length l = length k ->
-  exists l', l ≡ₚ l' /\
-  zip l k ≡ₚ zip l' k'.
-Proof.
-  intros Hk Hlen%eq_sym.
-  destruct (zip_Permutation_l_exists_r k k' l Hk Hlen) as (l' & Hl' & Hzip).
-  exists l'.
-  split; [easy|].
-  rewrite <- 2 (@zip_with_flip A B).
-  apply (fmap_Permutation prod_swap) in Hzip.
-  rewrite 2 fmap_zip_with in Hzip.
-  apply Hzip.
-Qed.
-
-
-
-
-(*
-Lemma input_edges_edges_perm_eq int_lab ints ints'
-  ext_lab exts exts' k :
-  ints ≡ₚ ints' -> exts ≡ₚ exts' ->
-  length int_lab = length ints ->
-  length ext_lab = length exts ->
-  input_edges (zip int_lab ints) (zip ext_lab exts) k ≡ₚ
-  input_edges (zip int_lab ints') (zip ext_lab exts') k.
-Proof.
-  intros Hints Hexts Hleni Hlene.
-  unfold input_edges.
-  f_equiv.
-  - rewrite 2 (list_fmap_compose fst).
-    unfold node_input_edges.
-    rewrite list_filter_fmap.
-    rewrite <- Combinators.compose_assoc.
-  intros Hlint Hlext Hleni Hlene.
-  specialize
-  unfold input_edges.
-  do 2 f_equiv;
-  unfold node_input_edges;
-  now f_equiv.
-Qed. *)
-
-(* Lemma input_edges_lab_perm_eq int_lab int_lab' ints
-  ext_lab ext_lab' exts k :
-  int_lab ≡ₚ int_lab' -> ext_lab ≡ₚ ext_lab' ->
-  length int_lab = length ints ->
-  length ext_lab = length exts ->
-  input_edges (zip int_lab ints) (zip ext_lab exts) k ≡ₚ
-  input_edges (zip int_lab' ints) (zip ext_lab' exts) k.
-Proof.
-  intros Hlint Hlext Hleni Hlene.
-  specialize
-  unfold input_edges.
-  do 2 f_equiv;
-  unfold node_input_edges;
-  now f_equiv.
-Qed. *)
-
-
-Lemma graph_namedtensorlist_semantics_aux_perm_eq' lint lint' lext lext' ks ks' :
-  NoDup lint.*1 -> lint ≡ₚ lint' ->
-  lext ≡ₚ lext' -> ks ≡ₚ ks' ->
-  graph_namedtensorlist_semantics_aux lint lext ks ≡ntl'≡ₚ
-  graph_namedtensorlist_semantics_aux lint' lext' ks'.
-Proof.
-  intros Hdup Hlint Hlext Hks.
-  split; cbn.
-  - apply list_to_map_proper; [|now f_equiv].
-    rewrite <- list_fmap_compose.
-    unfold compose; cbn.
-    change (_ <$> _) with (Pos.of_succ_nat ∘ fst <$> lint).
-    rewrite list_fmap_compose.
-    now apply (NoDup_fmap_2 _ _).
-  - etransitivity; [|apply (Permutation_PermutationA _); now rewrite <- Hks].
-    apply eqlistA_PermutationA.
-    apply eqlistA_altdef.
-    rewrite Forall2_fmap.
-    apply Forall_Forall2_diag, (set_Forall_list_to_set (C:=gset nat)).
-    intros k _.
-    now apply mk_node_perm_eq.
-Qed.
-
-(* FIXME: Move *)
-Lemma ntl_aeq_WF ntl ntl' :
-  ntl =ntl= ntl' -> WF_ntl ntl -> WF_ntl ntl'.
-Proof.
-  intros (fr & Hfr & Hfsums & Hfabs).
+  intros (fr & Hfrinj & Hsums & Habs & Hdelt).
+  exists fr.
+  rewrite abstracts_bound_vars_ntl_relabel_absidx,
+    deltas_bound_vars_ntl_relabel_absidx.
+  split; [apply Hfrinj|].
+  split; [apply Hsums|].
+  split; [|apply Hdelt].
   cbn.
-  intros [Hdup Habs].
-  split.
-  - rewrite <- Hfsums.
-    rewrite fsts_prod_map.
-    apply NoDup_fmap_2_strong, Hdup.
-    intros ? ? Hx Hy; apply Hfr; set_solver + Hx Hy.
-  - rewrite <- Hfsums, <- Hfabs.
-    rewrite abstracts_rel_vars_relabel_rels, fsts_prod_map,
-      <- (set_map_list_to_set_L (SA:=Pset)).
-    f_equiv; apply Habs.
+  rewrite <- Habs.
+  rewrite <- 2 list_fmap_compose.
+  apply eq_reflexivity, list_fmap_ext; now intros _ [[]] _.
 Qed.
-Lemma ntl_aeq_of_WF ntl ntl' : WF_ntl ntl ->
+
+
+Lemma graph_namedtensorlist_semantics_isomorphic {n m} (tg tg' : TensorGraph n m) :
+  isomorphic tg tg' ->
+  exists fv, Inj eq eq fv /\
+  ntl_relabel_absidx fv (graph_namedtensorlist_semantics tg) =ntl=
+  graph_namedtensorlist_semantics tg'.
+Proof.
+  intros (fe & fv & Hfe & Hfv & ->)%isomorphic_exists.
+  exists fv.
+  split; [easy|].
+  rewrite (graph_namedtensorlist_semantics_relabel_graph _),
+    (graph_namedtensorlist_semantics_reindex_graph _).
+  reflexivity.
+Qed.
+
+(* FIXME: Move *)
+(* Lemma ntl_aeq_of_WF ntl ntl' : WF_ntl ntl ->
   (exists fr,
     set_Forall2 (λ i j, fr i = fr j -> i = j) (list_to_set ntl.(ntl_sums).*1:>Pset ) /\
     prod_map fr id <$> ntl.(ntl_sums) ≡ₚ ntl'.(ntl_sums) /\
-    relabel_abs (relabel_rels fr) <$> ntl.(ntl_abstracts) ≡ₚ ntl'.(ntl_abstracts)
+    relabel_abs (relabel_bounds fr) <$> ntl.(ntl_abstracts) ≡ₚ ntl'.(ntl_abstracts)
     ) ->
   ntl =ntl= ntl'.
 Proof.
@@ -581,90 +521,9 @@ Proof.
   split; [|easy].
   intros x y Hx Hy.
   apply Hfr; specialize (HWF.2); [set_solver +Hx|set_solver +Hy].
-Qed.
+Qed. *)
 
 (* FIXME: Move *)
-
-Lemma graph_namedtensorlist_semantics_ppermute tg int_lab fi ext_lab :
-  NoDup int_lab -> length int_lab = num_internals tg ->
-  posperm (lengthP int_lab) fi ->
-  graph_namedtensorlist_semantics tg int_lab ext_lab =ntl=
-  graph_namedtensorlist_semantics tg (ppermute fi int_lab) ext_lab.
-Proof.
-  intros Hdup Hlen Hfi.
-  pose proof (lengthN_correct int_lab).
-  rewrite 2 graph_namedtensorlist_semantics_to_aux.
-  apply ntl_aeq_of_WF; [now rewrite <- graph_namedtensorlist_semantics_to_aux;
-    apply graph_namedtensorlist_semantics_WF|].
-
-
-  cbn.
-  rewrite (list_fmap_compose fst), fst_zip by now apply eq_reflexivity.
-  rewrite <- list_fmap_compose.
-  change (fst ∘ _) with (Pos.of_succ_nat).
-  rewrite (list_fmap_compose fst), fst_zip by
-    now rewrite length_ppermute; apply eq_reflexivity.
-  (* rewrite <- list_fmap_compose. *)
-  change (fst ∘ _) with (Pos.of_succ_nat).
-  pose proof (lengthN_correct int_lab).
-  exists (Pos.of_succ_nat
-      ∘ (λ x : Ty,
-           default x
-             (list_index x int_lab
-              ≫= λ i : Ty, int_lab !! (fi (Pos.of_succ_nat i):>nat)))
-      ∘ pos_to_nat_pred).
-  split_and!.
-  - intros _ _ (x & -> & Hx)%elem_of_list_to_set%elem_of_list_fmap
-      (y & -> & Hy)%elem_of_list_to_set%elem_of_list_fmap.
-    cbn.
-    rewrite 2 pos_to_nat_pred_of_nat.
-    apply elem_of_list_lookup in Hx as Hi.
-    apply elem_of_list_lookup in Hy as Hj.
-    destruct Hi as [i Hi], Hj as [j Hj].
-    apply list_index_Some_NoDup in Hi as Hi'; [|easy].
-    apply list_index_Some_NoDup in Hj as Hj'; [|easy].
-    rewrite Hi', Hj'.
-    cbn.
-    intros Heq%(inj Pos.of_succ_nat).
-    pose proof (posperm_bounded _ _ Hfi) as Hfibdd.
-    apply lookup_lt_Some in Hi as Hilt.
-    apply lookup_lt_Some in Hj as Hjlt.
-
-    assert (is_Some (int_lab !! (fi (Pos.of_succ_nat i) :> nat))) as Hfi_i. 1:{
-      apply lookup_lt_is_Some.
-      specialize (Hfibdd (Pos.of_succ_nat i)).
-      lia.
-    }
-    assert (is_Some (int_lab !! (fi (Pos.of_succ_nat j) :> nat))) as Hfi_j. 1:{
-      apply lookup_lt_is_Some.
-      specialize (Hfibdd (Pos.of_succ_nat j)).
-      lia.
-    }
-    destruct Hfi_i as [fii Hfii], Hfi_j as [fij Hfij].
-    rewrite Hfii, Hfij in Heq.
-    cbn in Heq.
-    subst fij.
-    specialize (NoDup_lookup _ _ _ _ Hdup Hfii Hfij)
-      as Heq%(inj pos_to_nat_pred).
-    apply (posperm_inj _ _ Hfi) in Heq as Heq%(inj _); [|lia..].
-    subst j.
-    congruence.
-  - rewrite ppermute_alt_list_index_total by now easy + apply posperm_bounded.
-    apply eq_reflexivity.
-    rewrite <- 2 list_fmap_compose.
-    apply list_fmap_ext; intros _ x Hx%elem_of_list_lookup_2.
-    cbn.
-    now rewrite pos_to_nat_pred_of_nat.
-  -
-    apply eq_reflexivity.
-    rewrite <- list_fmap_compose.
-    apply list_fmap_ext; intros _ k Hk%elem_of_list_lookup_2.
-    rewrite <- (elem_of_list_to_set (C:=gset nat)), <- dom_alt in Hk.
-    cbn [compose].
-    rewrite ppermute_alt_list_index_total by now easy + apply posperm_bounded.
-    rewrite zip_fmap_l, <- relabel_rels_mk_node.
-    reflexivity.
-Qed.
 
 Lemma NoDup_fmap_ind `(f : A -> B) (P : list A -> Prop)
   (Pnil : P []) (Pcons : forall a l, f a ∉ f <$> l -> NoDup (f <$> l) ->
@@ -676,181 +535,6 @@ Proof.
   intros []; eauto.
 Qed.
 
-Lemma input_edges_ext_label_irrel lint lext lext' k :
-  lext.*2 = lext'.*2 ->
-  input_edges lint lext k = input_edges lint lext' k.
-Proof.
-  intros Hlext.
-  unfold input_edges; f_equal.
-  unfold node_input_edges.
-  rewrite 2 (list_fmap_compose snd), <- 2 list_filter_fmap.
-  now rewrite Hlext.
-Qed.
-
-Lemma output_edges_ext_label_irrel lint lext lext' k :
-  lext.*2 = lext'.*2 ->
-  output_edges lint lext k = output_edges lint lext' k.
-Proof.
-  intros Hlext.
-  unfold output_edges; f_equal.
-  unfold node_output_edges.
-  rewrite 2 (list_fmap_compose snd (_ ∘ snd)), <- 2 list_filter_fmap.
-  now rewrite Hlext.
-Qed.
-
-Lemma mk_node_ext_label_irrel lint lext lext' k :
-  lext.*2 = lext'.*2 ->
-  mk_node lint lext k = mk_node lint lext' k.
-Proof.
-  intros Hext.
-  unfold mk_node.
-  f_equal; [f_equal|];
-  [now apply input_edges_ext_label_irrel|
-   now apply output_edges_ext_label_irrel].
-Qed.
-
-Lemma zip_with_irrel_l {A B C} (f : B -> C) (l l' : list A) (k : list B) :
-  length l = length l' ->
-  zip_with (λ _ b, f b) l k = zip_with (λ _ b, f b) l' k.
-Proof.
-  intros Hall%Forall2_same_length.
-  revert k;
-  induction Hall; intros []; cbn; congruence.
-Qed.
-
-Lemma zip_with_irrel_r {A B C} (f : A -> C) (l : list A) (k k' : list B) :
-  length k = length k' ->
-  zip_with (λ a _, f a) l k = zip_with (λ a _, f a) l k'.
-Proof.
-  intros Hall%Forall2_same_length.
-  revert l;
-  induction Hall; intros []; cbn; congruence.
-Qed.
-
-Lemma graph_namedtensorlist_semantics_ext_lab_irrel tg int_lab ext_lab ext_lab' :
-  length ext_lab = length ext_lab' ->
-  graph_namedtensorlist_semantics tg int_lab ext_lab =
-  graph_namedtensorlist_semantics tg int_lab ext_lab'.
-Proof.
-  intros Hlen.
-  unfold graph_namedtensorlist_semantics.
-  f_equal.
-  apply list_fmap_ext; intros _ x _.
-  apply mk_node_ext_label_irrel.
-  rewrite 2 fmap_zip_with; cbn.
-  now apply zip_with_irrel_l.
-Qed.
-
-
-
-Lemma graph_namedtensorlist_semantics_perm_eq tg int_lab int_lab'
-  ext_lab ext_lab' :
-  NoDup int_lab -> length int_lab = num_internals tg ->
-  int_lab ≡ₚ int_lab' ->
-  length ext_lab = length ext_lab' ->
-  graph_namedtensorlist_semantics tg int_lab ext_lab =ntl=
-  graph_namedtensorlist_semantics tg int_lab' ext_lab'.
-Proof.
-  intros Hdup Hlen (f & Hf & <- & Hlook)%perm_exists_posperm Hext.
-  etransitivity; [apply graph_namedtensorlist_semantics_ppermute; eauto|].
-  apply eq_reflexivity.
-  now apply graph_namedtensorlist_semantics_ext_lab_irrel.
-Qed.
-
-
-Lemma graph_namedtensorlist_semantics_seq_correct' tg :
-  graph_tensorlist_semantics tg =
-  ntl2tl (graph_namedtensorlist_semantics tg (seq 0 (num_internals tg))
-	  (seq 0 (num_externals tg))).
-Proof.
-  rewrite graph_namedtensorlist_semantics_seq_correct.
-  now rewrite tl2ntl2tl.
-Qed.
-
-Lemma internal_edges_perm ns es es' :
-  es ≡ₚ es' ->
-  @internal_edges T (mk_tg ns es) ≡ₚ internal_edges (mk_tg ns es').
-Proof.
-  intros Hes.
-  unfold internal_edges; cbn.
-  now f_equiv.
-Qed.
-
-Lemma external_edges_perm ns es es' :
-  es ≡ₚ es' ->
-  @external_edges T (mk_tg ns es) ≡ₚ external_edges (mk_tg ns es').
-Proof.
-  intros Hes.
-  unfold external_edges; cbn.
-  now f_equiv.
-Qed.
-
-
-Lemma graph_tensorlist_semantics_perm_eq_pairs_elab ns es es' :
-  es ≡ₚ es' ->
-  exists idxs idxs',
-  idxs ≡ₚ seq 0 (num_internals (mk_tg ns es)) /\
-  idxs' ≡ₚ seq 0 (num_externals (mk_tg ns es)) /\
-  tl2ntl (graph_tensorlist_semantics (mk_tg ns es)) ≡ntl'≡ₚ
-  graph_namedtensorlist_semantics_aux
-    (zip idxs (internal_edges (mk_tg ns es')))
-    (zip idxs' (external_edges (mk_tg ns es')))
-    (map_to_list ns).*1 /\
-  graph_namedtensorlist_semantics_aux
-    (zip idxs (internal_edges (mk_tg ns es')))
-    (zip idxs' (external_edges (mk_tg ns es')))
-    (map_to_list ns).*1
-    =ntl= tl2ntl (graph_tensorlist_semantics (mk_tg ns es')).
-Proof.
-  intros Hes.
-  apply (internal_edges_perm ns) in Hes as Hies.
-  apply (external_edges_perm ns) in Hes as Hees.
-
-  apply perm_exists_perm_seq in Hies as Hidxs.
-  apply perm_exists_perm_seq in Hees as Hidxs'.
-
-  destruct Hidxs as (idxs & Hidxs & Himap).
-  destruct Hidxs' as (idxs' & Hidxs' & Himap').
-  exists idxs, idxs'.
-  split; [easy|].
-  split; [easy|].
-  split.
-  - rewrite <- graph_namedtensorlist_semantics_seq_correct.
-    rewrite graph_namedtensorlist_semantics_to_aux.
-    cbn [nodes].
-    eapply graph_namedtensorlist_semantics_aux_perm_eq';
-    [rewrite fst_zip by (now rewrite length_seq);
-     apply NoDup_seq|..|reflexivity].
-    + etransitivity; [|apply Himap].
-      now rewrite imap_to_zip_with_seq.
-    + etransitivity; [|apply Himap'].
-      now rewrite imap_to_zip_with_seq.
-  - rewrite <- graph_namedtensorlist_semantics_to_aux.
-    rewrite <- graph_namedtensorlist_semantics_seq_correct.
-    apply graph_namedtensorlist_semantics_perm_eq.
-    + rewrite Hidxs; apply NoDup_seq.
-    + rewrite Hidxs.
-      now rewrite length_seq, Hies.
-    + rewrite Hidxs.
-      f_equiv.
-      now rewrite Hies.
-    + rewrite Hidxs'.
-      now rewrite 2 length_seq, Hees.
-Qed.
-
-
-Lemma graph_tensorlist_semantics_perm_eq_pairs ns es es' :
-  es ≡ₚ es' ->
-  exists mid,
-  tl2ntl (graph_tensorlist_semantics (mk_tg ns es)) ≡ntl'≡ₚ mid /\
-  mid =ntl= tl2ntl (graph_tensorlist_semantics (mk_tg ns es')).
-Proof.
-  intros Hes.
-  apply (graph_tensorlist_semantics_perm_eq_pairs_elab ns) in Hes.
-  naive_solver.
-Qed.
-
- *)
 
 
 
