theories/GraphCore/TensorGraphSemantics.v
@@ -1,68 +1,53 @@
 Require Export TensorGraphExpr.
-Require Export TensorExprDBSemantics.
+Require Export TESemantics.
 
 (* Semantics of tensor graphs into (semi)rings, via tensor expressions *)
-
+(* FIXME: Move*)
+Fixpoint vseq (start len : nat) : vec nat len :=
+  match len with 
+  | O => [#]
+  | S len => start ::: vseq (S start) len
+  end.
+Lemma vec_to_list_seq start len : 
+  vec_to_list (vseq start len) = seq start len.
+Proof.
+  revert start; induction len; intros start; cbn; f_equal; done.
+Qed.
 
 Section TensorGraphSemantics.
 
 Context {R A T : Type}.
 
-Let TensorGraph := (TensorGraph T).
-
-Implicit Types tg : TensorGraph.
-
-Definition graph_V : nat -> Type := fun _ => A.
-Definition graph_Vsum `{Summable A} : forall k, Summable (graph_V k)
-  := fun _ => _.
+Let TensorGraph := (CospanHyperGraph T).
 
 
 
 (* Combine input and output maps to get the local variable map *)
 Definition graph_ml (minput : gmap nat A) (moutput : gmap nat A) :
-  Pmap (Vval graph_V) :=
-  @mk_Vval graph_V 0 <$> gmaps_to_Pmap minput moutput.
+  Pmap A := gmaps_to_Pmap minput moutput.
 
+Definition graph_mabs `{TensorLike R A T}
+  (tm : Pmap (T * list positive * list positive)) : Pmap (@DimensionlessTensor R A) :=
+  interpretTensor ∘ fst ∘ fst <$> tm.
 
-Definition graph_tensor_to_V_n_args
-  {n m} (t : vec A n -> vec A m -> R) :=
-  tensor_to_V_n_args_aux graph_V 0 (uncurry t ∘ Vector.splitat n).
-
-
-
-Definition graph_mabs `{TensorLike R A T} 
-  (tg : TensorGraph) : Pmap (@Vfunc R graph_V) :=
-  kmap (Pos.of_succ_nat) $ map_imap (fun k (dt : T) =>
-    (* let node := mk_node (i_internal_edges tg) (i_external_edges tg) n in *)
-    let inarity := in_arity tg.2 k in
-    let outarity := out_arity tg.2 k in
-    Some $ mk_Vfunc graph_V (replicate (inarity + outarity) O)
-      (graph_tensor_to_V_n_args (interpretTensor dt inarity outarity))
-    ) tg.1.
-
-Definition graph_map_semantics 
-  `{SR : SemiRing R rO rI radd rmul req} `{!Summable A} `{TensT : TensorLike R A T}
-  (tg : TensorGraph)
+Definition graph_map_semantics `{SR : SemiRing R rO rI radd rmul req} 
+  `{!Summable A, !EqDecision A} `{TensT : TensorLike R A T}
+  {n m} (tg : TensorGraph n m)
   (minput : gmap nat A) (moutput : gmap nat A) : R :=
-  tl_total_semantics (SR:=SR) graph_V (Vsum:=graph_Vsum)
-    (graph_mabs tg)
-    ∅
+  ntl_total_semantics (SR:=SR)
+    (graph_mabs tg.(hedges))
     (graph_ml minput moutput)
-    (graph_tensorlist_semantics tg).
+    (graph_namedtensorlist_semantics tg).
 
 
 
+Definition graph_semantics `{SR : SemiRing R rO rI radd rmul req} 
+  `{!Summable A, !EqDecision A} `{TensT : TensorLike R A T}
+  {n m} (tg : TensorGraph n m) : @Tensor R n m A :=
+  namedtensorlist_to_tensor (SR:=SR) (graph_mabs tg.(hedges))
+    (vmap (bcons false ∘ Pos.of_succ_nat) (vseq 0 n)) 
+    (vmap (bcons true ∘ Pos.of_succ_nat) (vseq 0 m))
+    (graph_namedtensorlist_semantics tg).
 
-Definition graph_list_semantics 
-  `{SR : SemiRing R rO rI radd rmul req} `{!Summable A} `{TensT : TensorLike R A T}
-  (tg : TensorGraph) (ins : list A) (outs : list A) : R :=
-  graph_map_semantics tg
-    (list_to_map $ zip (sorted_inputs tg) ins)
-    (list_to_map $ zip (sorted_outputs tg) outs).
-
-Definition graph_vector_semantics 
-  `{SR : SemiRing R rO rI radd rmul req} `{!Summable A} `{TensT : TensorLike R A T}
-  (tg : TensorGraph) (ins : vec A (graph_insize tg)) (outs : vec A (graph_outsize tg)) : R :=
-  graph_list_semantics tg (vec_to_list ins) (vec_to_list outs).
 
 End TensorGraphSemantics.
